theories/Equiv/SimDivergence.v
@@ -1,0 +1,43 @@
+Require Import List.
+Require Import Util Var Val Exp Envs Map CSet AutoIndTac IL AllInRel.
+Require Import SmallStepRelations StateType Sim Divergence.
+
+Set Implicit Arguments.
+Unset Printing Records.
+
+Lemma sim_diverge {S} `{StateType S} {S'} `{StateType S'} (σ:S) (σ':S')
+  : sim bot3 Sim σ σ'
+    -> div bot1 σ'
+    -> ~ (exists σ'', star2 step σ nil σ'' /\ normal2 step σ'' /\ result σ'' = None)
+    -> div bot1 σ.
+Proof.
+  revert σ σ'. pcofix CIH; intros.
+  pinversion H2; subst.
+  - eapply plus2_destr_nil in H1; dcr.
+    pfold. econstructor; eauto.
+    right. eapply CIH; eauto.
+    eapply sim_expansion_closed; eauto using plus2_star2.
+    intro; eapply H4; dcr; eexists; split; eauto.
+    eapply (star2_step EvtTau); eauto.
+  - eapply div_diverges in H3.
+    exfalso.
+    eapply diverges_never_activated in H7; eauto.
+    eapply diverges_reduction_closed; eauto using plus2_star2.
+  - exfalso. eapply H4.
+    eauto.
+  - eapply div_diverges in H3.
+    exfalso. eapply diverges_never_terminates; eauto.
+    eapply diverges_reduction_closed; eauto using plus2_star2.
+Qed.
+
+Lemma sim_complete_diverges S `{StateType S} S' `{StateType S'} (σ:S) (σ':S') p r
+: diverges σ -> diverges σ' -> sim r p σ σ'.
+Proof.
+  revert σ σ'. pcofix COH; intros.
+  inv H2; inv H3.
+  pfold.
+  econstructor.
+  - econstructor; eauto.
+  - econstructor; eauto.
+  - right. eapply COH; eauto.
+Qed.
