theories/Equiv/SimRel.v
@@ -1,0 +1,39 @@
+Require NonParametricBiSim.
+Require Import Sim SimLockStep IL paco3 OptionR.
+Require Export ILStateType BlockType ILProperties.
+
+Lemma bisim_sim S `{StateType S} S' `{StateType S'} (σ:S) (σ':S')
+  : sim bot3 Bisim σ σ'
+    -> sim bot3 SimExt σ σ'.
+Proof.
+  revert σ σ'.
+  pcofix CIH.
+  intros. pinversion H2; subst; pfold.
+  - econstructor; try eassumption.
+    right. eapply CIH. eauto.
+  - econstructor 2; try eassumption.
+    + intros. edestruct H6; eauto; dcr; pclearbot.
+      eexists; split; eauto.
+    + intros. edestruct H7; eauto; dcr; pclearbot.
+      eexists; split; eauto.
+  - econstructor 3; try eassumption. eauto.
+  - econstructor 4; try eassumption.
+Qed.
+
+Lemma sim_ext_sim S `{StateType S} S' `{StateType S'} (σ:S) (σ':S')
+  : sim bot3 SimExt σ σ'
+    -> sim bot3 Sim σ σ'.
+Proof.
+  revert σ σ'.
+  pcofix CIH.
+  intros. pinversion H2; subst; pfold.
+  - econstructor; try eassumption.
+    right. eapply CIH. eauto.
+  - econstructor 2; try eassumption.
+    + intros. edestruct H6; eauto; dcr; pclearbot.
+      eexists; split; eauto.
+    + intros. edestruct H7; eauto; dcr; pclearbot.
+      eexists; split; eauto.
+  - econstructor 3; try eassumption.
+  - econstructor 4; try eassumption.
+Qed.
