theories/ValueOpts/ValueOpts.v
@@ -88,88 +88,10 @@ Proof.
     rewrite <- H3; eauto.
 Qed.
 
-
-Instance subst_exp_Proper Z Y
-  : Proper (_eq ==> _eq) (subst_op (sid [Z <-- Y])).
-Proof.
-  hnf; intros. inv H. clear H.
-  simpl. general induction y; simpl; eauto.
-Qed.
-
 Ltac dowith c t :=
   match goal with
     | [ H : c _ _ _ _ |- _ ] => t H
   end.
-
-Lemma eval_op_subst E y Y Z e
-: length Z = length Y
-  -> omap (op_eval E) Y = ⎣y ⎦
-  -> op_eval (E [Z <-- List.map Some y]) e =
-    op_eval E (subst_op (sid [Z <-- Y]) e).
-Proof.
-  intros.
-  general induction e; simpl; eauto.
-  - eapply length_length_eq in H.
-    general induction H; simpl in * |- *; eauto.
-    monad_inv H0. simpl.
-    lud; eauto.
-  - erewrite IHe; eauto.
-  - erewrite IHe1; eauto.
-    erewrite IHe2; eauto.
-Qed.
-
-Lemma satisfies_subst V Z Y y bE gamma
-  (EVAL: omap (op_eval V) Y = ⎣ y ⎦)
-  (Len1 : ❬Y❭ = ❬y❭)
-  (Len2 : ❬Z❭ = ❬Y❭)
-  (AGR:agree_on eq (freeVars gamma \ of_list Z) V bE)
-  : satisfies V (subst_eqn (sid [Z <-- Y]) gamma) <-> satisfies (bE [Z <-- Some ⊝ y]) gamma.
-Proof.
-  destruct gamma; simpl in *.
-  * do 2 rewrite <- (eval_op_subst _ _ _ _ Len2 EVAL); eauto.
-    erewrite op_eval_agree; [| |reflexivity].
-    erewrite op_eval_agree with (e:=e'); [| |reflexivity].
-    reflexivity.
-    -- eapply update_with_list_agree; eauto with len.
-       symmetry.
-       eapply agree_on_incl; eauto. cset_tac.
-    -- eapply update_with_list_agree; eauto with len.
-       symmetry.
-       eapply agree_on_incl; eauto.
-       cset_tac.
-  * simpl in * |- *.
-    do 2 erewrite <- (eval_op_subst _ _ _ _ Len2 EVAL); eauto.
-    erewrite op_eval_agree; [| |reflexivity].
-    erewrite op_eval_agree with (e:=e'); [| |reflexivity]; eauto.
-    reflexivity.
-    -- eapply update_with_list_agree; eauto with len.
-       symmetry.
-       eapply agree_on_incl; eauto.
-       cset_tac.
-    -- eapply update_with_list_agree; eauto with len.
-       symmetry.
-       eapply agree_on_incl; eauto.
-       cset_tac.
-  * reflexivity.
-Qed.
-
-Lemma satisfiesAll_subst V Z EqS Y y bE
-:  omap (op_eval V) Y = ⎣y⎦
-   -> agree_on eq (eqns_freeVars EqS \ of_list Z) V bE
-   -> length Z = length Y
-   -> satisfiesAll V (subst_eqns (sid [Z <-- Y]) EqS) <-> satisfiesAll (bE [Z <-- List.map Some y]) EqS.
-Proof.
-  revert_except EqS. pattern EqS. eapply set_induction; intros.
-  - hnf; intros. eapply empty_is_empty_1 in H.
-    rewrite H. rewrite subst_eqns_empty.
-    unfold satisfiesAll; split; intros; cset_tac.
-  - eapply Add_Equal in H1. rewrite H1 in *.
-    rewrite subst_eqns_add.
-    rewrite !satisfiesAll_add.
-    rewrite eqns_freeVars_add in H3.
-    rewrite satisfies_subst; eauto with len;[|eauto with cset].
-    rewrite H; eauto with cset. reflexivity.
-Qed.
 
 Lemma eqn_sound_entails_monotone ZL Δ Γ1 Γ1' s s' ang
   : renamedApart s ang
